changed college.bpl

college.bpl
@@ -1,17 +1,17 @@
 var collegeNumber :[Ref]int;
-var numberBuildings : [Ref]int;
+var endowment : [Ref]int;
 
 var packedCollegeNumberField : [Ref]bool;
 var fracCollegeNumberField : [Ref]real;
 
-var packedNumberBuildingsField : [Ref]bool;
-var fracNumberBuildingsField : [Ref]real;
+var packedCollegeFacilitiesMany : [Ref]bool;
+var fracCollegeFacilitiesMany : [Ref]real;
 
-var packedCollegeBuildingsMany : [Ref]bool;
-var fracCollegeBuildingsMany : [Ref]real;
+var packedCollegeFacilitiesFew : [Ref]bool;
+var fracCollegeFacilitiesFew : [Ref]real;
 
-var packedCollegeBuildingsFew : [Ref]bool;
-var fracCollegeBuildingsFew : [Ref]real;
+var packedCollegeFields : [Ref]bool;
+var fracCollegeFields : [Ref]real;
 
 procedure PackCollegeNumberField(c: int, this:Ref);
 requires (packedCollegeNumberField[this]==false) &&
@@ -21,12 +21,86 @@ procedure UnpackCollegeNumberField(c: int, this:Ref);
 requires packedCollegeNumberField[this];
 ensures	(collegeNumber[this] == c);
 
+procedure PackCollegeFields(c: int, e:int, this:Ref);
+requires (packedCollegeFields[this]==false) &&
+ 	(collegeNumber[this] == c) && (endowment[this] == e); 
 
-predicate collegeBuildingsMany() = 
-	exists c:int, n:int ::
-		(this.collegeNumber -> c) && (this.numberBuildings -> n) && 
-		(n == 10 * c)
-		
-predicate collegeBuildingsFew() = exists c:int, n:int ::
-	(this.collegeNumber -> c) && (this.numberBuildings -> n) && (n == 4 * c) 
+procedure UnpackCollegeFields(c: int, e:int, this:Ref);
+requires packedCollegeFields[this];
+ensures	(collegeNumber[this] == c);
+ensures (endowment[this] == e);
 
+procedure PackCollegeFacilitiesMany(num:int, c:int, this:Ref);
+requires (packedCollegeFacilitiesMany[this] == false);
+//TODO all Pack procedures need to refer to frac also, 
+// not only to packed.
+requires (collegeNumber[this] == c) && (num >= 10 * c);
+
+procedure UnpackCollegeFacilitiesMany(num:int, c:int, this:Ref);
+requires packedCollegeFacilitiesMany[this];
+//TODO all Unpack procedures need to refer to frac also, 
+// not only to packed.
+ensures (collegeNumber[this] == c) && (num >= 10 * c);
+
+procedure PackCollegeFacilitiesFew(num:int, c:int, this:Ref);
+requires (packedCollegeFacilitiesFew[this] == false);
+requires (collegeNumber[this] == c) && (num <= 4 * c);
+
+procedure UnpackCollegeFacilitiesFew(num:int, c:int, this:Ref);
+requires packedCollegeFacilitiesFew[this];
+ensures (collegeNumber[this] == c) && (num <= 4 * c);
+
+procedure ConstructCollege(number:int, this:Ref) 
+modifies collegeNumber, endowment;
+ensures packedCollegeFields[this] &&
+	(fracCollegeFields[this] == 1.0);
+// TODO need to put in statements about the parameters.
+// ensures this#1.0 CollegeFields()[number, (number*1000)-5]
+{
+	collegeNumber[this] := number;
+	endowment[this] := (number *1000) - 5;
+}
+
+procedure getCollegeNumber(this:Ref) returns (r:int)
+ensures packedCollegeNumberField[this] &&
+	(fracCollegeNumberField[this] == 1.0);
+// TODO add statement about value of parameter 
+// ensures this#1.0 CollegeNumberField()[result]
+{
+	r := collegeNumber[this];
+}
+
+// the method that calculates the extrinsic state
+procedure getNumberFacilities(int campusNumber) returns (r:Ref)
+requires packedCollegeNumberField[this] && 
+	(fracCollegeNumberField[this] == 1.0);
+//TODO have to say what are the current values of the parameters
+// requires this#1 CollegeNumberField(this.collegeNumber)
+ensures packedMultipleOf[r] &&
+	(fracMultipleOf[r] == 1.0);
+//ensures result#1 MultipleOf(this.collegeNumber)
+{
+	call ConstructIntCell(collegeNumber[this] * campusNumber, r);
+}
+
+procedure checkFewFacilities(num:int) returns (b:bool)
+requires packedCollegeFacilitiesFew[this] &&
+	(fracCollegeFacilitiesFew[this] == 1.0);
+//requires this#1 collegeFacilitiesFew(num)
+ensures packedCollegeFacilitiesFew[this] &&
+	(fracCollegeFacilitiesFew[this] == 1.0);
+//ensures this#1 collegeFacilitiesFew(num)
+{
+	r := (num <= 4 * collegeNumber[this]);
+}
+
+procedure checkManyFacilities(int num) returns (b:bool)
+requires packedCollegeFacilitiesMany[this] &&
+	(fracCollegeFacilitiesMany[this] == 1.0);
+//requires this#1 collegeFacilitiesMany(num)
+ensures packedCollegeFacilitiesMany[this] &&
+	(fracCollegeFacilitiesMany[this] == 1.0);
+//ensures this#1 collegeFacilitiesMany(num)
+{
+	r := (num >= 10 * collegeNumber[this]);
+}
